theories/L6_PCPS/closure_conversion_corresp.v
@@ -1,0 +1,1734 @@
+Require Import cps cps_util set_util identifiers ctx alpha_conv hoare
+        Ensembles_util List_util closure_conversion closure_conversion_correct.
+Require Import Coq.ZArith.Znumtheory Coq.Relations.Relations Coq.Arith.Wf_nat.
+Require Import Coq.Lists.List Coq.MSets.MSets Coq.MSets.MSetRBT Coq.Numbers.BinNums
+        Coq.NArith.BinNat Coq.PArith.BinPos Coq.Sets.Ensembles Omega.
+Require Import ExtLib.Structures.Monads ExtLib.Data.Monads.StateMonad.
+
+Import ListNotations.
+
+Open Scope ctx_scope.
+Open Scope alpha_scope.
+
+
+(** * Correspondance of the relational and the computational definitions of  closure conversion *)
+
+Section CC_correct.
+  Context (utag : tag) (* Tag for types with unique constructor *)
+          (env_tag : tag) (* Tag for the type of environments *)
+          (tag_bij : tag -> tag) (* mapping from function tags to closure 
+                                    records tags *)
+          (unknown_type : type).
+
+
+  Open Scope ctx_scope.
+
+  (** All the variables greater or equal to x are in S (i.e. the "fresh" set) *)
+  Definition fresh (S : Ensemble var) (x : var) :=
+    forall y, (x <= y)%positive -> In _ S y.
+
+  (** Free variable map invariant *)
+  Definition FVmap_inv (FVmap : VarInfoMap) Scope Funs FVs : Prop :=
+    Same_set _ Scope (fun x => exists t, M.get x FVmap = Some (BoundVar t)) /\
+    Same_set _ (Setminus _ Funs Scope)
+             (fun x => exists x' t t', M.get x FVmap = Some (MRFun x' t t')) /\
+    forall N x, (nthN FVs N = Some x /\ ~ In _ Scope x /\ ~ In _ Funs x) <->
+           (exists t, M.get x FVmap = Some (FVar N t)).
+
+  (** Function names substitution *)
+  Definition subst (FVmap : VarInfoMap) x : var :=
+    match M.get x FVmap with
+      | Some (MRFun x' _ _) => x'
+      | _ => x
+    end.
+
+  Opaque bind ret.
+
+  (** A function that corresponds to an evaluation context *)
+  Definition is_exp_ctx (f : exp -> exp) C : Prop := 
+    forall e, f e = app_ctx_f C e. 
+
+  (** Set of variables not in the map *)
+  Definition binding_not_in_map {A} (S : Ensemble M.elt) (map : M.t A) := 
+    forall x : M.elt, In M.elt S x -> M.get x map = None.
+
+  (** Spec for [get_name] *)
+  Lemma get_name_fresh S :
+    {{ fun s => fresh S (fst s) }}
+      get_name
+    {{ fun _ x s' => fresh S x /\ fresh (Setminus var S (Singleton var x)) (fst s') }}.  
+  Proof.   
+    eapply pre_post_mp_l.
+    eapply bind_triple. eapply get_triple.
+    intros [x d] [x' d'].
+    eapply pre_post_mp_l. eapply bind_triple.
+    eapply put_triple. intros u [x'' d'']. eapply return_triple.
+    intros [x''' d'''] Heq1 [Heq2 Heq3] H. inv Heq1. inv Heq2. inv Heq3. 
+    split; eauto. intros y Hleq.
+    constructor.
+    - eapply H. simpl in *. zify. omega.
+    - intros Hin. inv Hin. simpl in *. eapply Pos.le_nlt in Hleq.
+      eapply Hleq. zify. omega.
+  Qed.
+  
+  Lemma fresh_monotonic S S' x :
+    Included _ S S' ->
+    fresh S x ->
+    fresh S' x.
+  Proof.
+    intros Hinc Hf x' Hleq. eapply Hinc. eapply Hf. eassumption.
+  Qed.
+
+  Definition f_eq_subdomain {A B} S (f1 f2 : A -> B) :=
+    forall x, In _ S x -> f1 x = f2 x.
+  
+
+  Lemma FVmap_inv_set_bound FVmap Scope Funs FVs x t :
+    FVmap_inv FVmap Scope Funs FVs ->
+    FVmap_inv (M.set x (BoundVar t) FVmap) (Union _ (Singleton _ x) Scope) Funs FVs.
+  Proof. 
+    intros [H1 [H2 H3]]. repeat split.
+    - intros y Hin. destruct (Coqlib.peq y x); subst.
+      + eexists. now rewrite M.gsspec, Coqlib.peq_true.
+      + inv Hin. inv H; congruence.
+        eapply H1 in H. edestruct H as [t' Heq].
+        eexists.  rewrite M.gsspec, Coqlib.peq_false; eauto.
+    - intros y Hin. destruct (Coqlib.peq y x); subst.
+      + eauto.
+      + edestruct Hin as [t' Heq]. rewrite M.gsspec, Coqlib.peq_false in Heq; [| now eauto ].
+        right. eapply H1. eexists; eauto.
+    - intros y Hin. inv Hin. destruct (Coqlib.peq y x); subst.
+      + exfalso. eauto.
+      + edestruct H2 as [H2' _].
+        edestruct H2' as [x' [t' [t'' Heq]]].
+        * constructor; eauto.
+        * eexists.  rewrite M.gsspec, Coqlib.peq_false; eauto.
+    - eapply H2. destruct H as [x' [t' [t'' Heq]]].
+      destruct (Coqlib.peq x x0); subst.
+      + rewrite M.gsspec, Coqlib.peq_true in Heq. congruence.
+      + repeat eexists. rewrite M.gsspec, Coqlib.peq_false in Heq; eauto.
+    - intros Hc. destruct H as [x' [t' [t'' Heq]]].
+      destruct (Coqlib.peq x0 x); subst.
+      + rewrite M.gsspec, Coqlib.peq_true in Heq. congruence.
+      + inv Hc. inv H; congruence.
+        eapply H2; eauto. repeat eexists.
+        rewrite M.gsspec, Coqlib.peq_false in Heq; eauto.
+    - intros [Hnth [Hnin Hnin']].
+      destruct (Coqlib.peq x0 x); subst.
+      + exfalso. eauto. 
+      + edestruct H3 as [[t' Heq] _].
+        now repeat split; eauto.
+        eexists. rewrite M.gsspec, Coqlib.peq_false; eauto.
+    - edestruct H as [t' Heq]. 
+      destruct (Coqlib.peq x0 x); subst.
+      + rewrite M.gsspec, Coqlib.peq_true in Heq. congruence.
+      + eapply H3; eauto.
+        rewrite M.gsspec, Coqlib.peq_false in Heq; eauto.
+    - edestruct H as [t' Heq]. 
+      destruct (Coqlib.peq x0 x); subst.
+      + rewrite M.gsspec, Coqlib.peq_true in Heq. congruence.
+      + intros Hc. inv Hc. inv H0; congruence.
+        rewrite M.gsspec, Coqlib.peq_false in Heq; eauto.
+        edestruct H3 as [_ [_ [Hc _]]].
+        eapply H3 in H0; eauto. contradiction.
+    - edestruct H as [t' Heq]. 
+      destruct (Coqlib.peq x0 x); subst.
+      + rewrite M.gsspec, Coqlib.peq_true in Heq. congruence.
+      + intros Hc.
+        rewrite M.gsspec, Coqlib.peq_false in Heq; eauto.
+        edestruct H3 as [_ [_ [_ Hc']]].
+        eapply H3 in Hc; eauto. contradiction.
+  Qed.
+
+  Lemma FVmap_inv_set_funs FVmap Scope Funs FVs x x' t t' :
+    ~ In _ Scope x ->
+    FVmap_inv FVmap Scope Funs FVs ->
+    FVmap_inv (M.set x (MRFun x' t t') FVmap) Scope (Union _ (Singleton _ x) Funs) FVs.
+  Proof. 
+    intros Hnin [H1 [H2 H3]]. repeat split.
+    - intros y Hin. destruct (Coqlib.peq y x); subst.
+      + contradiction.
+      + eapply H1 in Hin. edestruct Hin as [t'' Heq].
+        eexists.  rewrite M.gsspec, Coqlib.peq_false; eauto.
+    - intros y Hin. destruct (Coqlib.peq y x); subst.
+      + edestruct Hin as [t'' Heq]. rewrite M.gss in Heq; congruence.
+      + edestruct Hin as [t'' Heq]. rewrite M.gso in Heq; [| now eauto ].
+        eapply H1. eexists; eauto.
+    - intros y Hin. inv Hin. destruct (Coqlib.peq y x); subst.
+      + repeat eexists. rewrite M.gss. reflexivity.
+      + edestruct H2 as [H2' _].
+        edestruct H2' as [x'' [t'' [t''' Heq]]].
+        inv H. inv H4; congruence. constructor; eassumption.
+        repeat eexists. rewrite M.gso; eassumption.
+    - destruct (Coqlib.peq x0 x); subst; eauto. right.
+      eapply H2. edestruct H as [x'' [t1 [t2 Hget]]].
+      rewrite M.gso in Hget; [| now eauto ].
+      repeat eexists; eauto. 
+    - destruct H as [x'' [t1 [t2 Hget]]].
+      destruct (Coqlib.peq x0 x); subst; eauto.
+      rewrite M.gso in Hget; [| now eauto ].
+      intros Hc. apply H1 in Hc. edestruct Hc as [t3 Hget']. congruence.
+    - intros [Hnth [Hnin1 Hnin2]].
+      destruct (Coqlib.peq x0 x); subst.
+      + exfalso. eauto.
+      + edestruct H3 as [[t1 Heq] _].
+        now repeat split; eauto.
+        eexists. rewrite M.gsspec, Coqlib.peq_false; eauto.
+    - edestruct H as [t1 Heq].
+      destruct (Coqlib.peq x0 x); subst.
+      + rewrite M.gsspec, Coqlib.peq_true in Heq. congruence.
+      + eapply H3; eauto.
+        rewrite M.gsspec, Coqlib.peq_false in Heq; eauto.
+    - edestruct H as [t1 Heq].
+      destruct (Coqlib.peq x0 x); subst.
+      + rewrite M.gss in Heq. congruence.
+      + intros Hc.
+        rewrite M.gso in Heq; eauto. eapply H1 in Hc. 
+        edestruct Hc as [t2 Heq']. congruence.
+    - edestruct H as [t1 Heq].
+      destruct (Coqlib.peq x0 x); subst.
+      + rewrite M.gss in Heq. congruence.
+      + intros Hc.
+        rewrite M.gso in Heq; eauto.
+        inv Hc. inv H0; congruence.
+        edestruct H2 as [H2' _].  edestruct (H2' x0) as [y [t2 [t3 Hge']]].
+        constructor. eauto. intros Hc. eapply H1 in Hc. 
+        edestruct Hc as [t2 Heq']. congruence.
+        congruence.
+  Qed.
+
+  (** Spec for [get_var] *)
+  Lemma get_var_project_var_sound Scope Funs Γ FVs FVmap S x :
+    binding_in_map (Singleton _ x) FVmap ->
+    (* binding_not_in_map (Union _ S (Singleton _ Γ)) FVmap -> *)
+    FVmap_inv FVmap Scope Funs FVs ->
+    {{ fun s => fresh S (fst s) }}
+      get_var utag x FVmap Γ
+    {{ fun _ t s' =>
+         exists C S', 
+           fresh S' (fst s') /\
+           let '(x', _, f) := t in
+           project_var Scope Funs (subst FVmap) Γ FVs S x x' C S' /\
+           is_exp_ctx f C }}.
+  Proof.
+    intros Hin Minv. destruct Minv as [Minv1 [Minv2 Minv3]]. 
+    unfold get_var. edestruct (Hin x) as [inf Hget]; eauto. 
+    destruct inf; rewrite Hget. 
+    - eapply bind_triple.
+      + eapply get_name_fresh.     
+      + intros x' s. eapply return_triple. intros s' [Hf Hf'].
+        eexists (Eproj_c x' t n Γ Hole_c). repeat eexists. 
+        * eassumption.
+        * edestruct Minv3 as [H1 [H2 [H3 H4]]]. now repeat eexists; eauto.
+          econstructor 3; eauto.
+          eapply Hf. zify; omega.
+    - eapply bind_triple.
+      + eapply get_name_fresh.  
+      + intros x' s. eapply return_triple. intros s' [Hf Hf'].
+        edestruct Minv2 as [H1 H2]; eauto. 
+        exists (Econstr_c x' t0 utag [v; Γ] Hole_c). repeat eexists.
+        * eassumption.
+        * replace v with ((subst FVmap) x)
+            by (unfold subst; rewrite Hget; reflexivity). 
+          econstructor; eauto.
+          intros Hc. eapply Minv1 in Hc. destruct Hc as [t' Heq]. congruence.
+          eapply H2. repeat eexists; eauto.
+          eapply Hf. zify; omega.    
+    - eapply return_triple. intros [s d] Hin'.      
+      exists Hole_c. repeat eexists. 
+      + eassumption. 
+      + constructor. eapply Minv1. eexists; eauto.
+  Qed.
+  
+  (** Spec for [get_vars] *)
+  Lemma get_vars_project_vars_sound Scope Funs Γ FVs FVmap S xs :
+    binding_in_map (FromList xs) FVmap ->
+    FVmap_inv FVmap Scope Funs FVs ->
+    {{ fun s => fresh S (fst s) }}
+      get_vars utag xs FVmap Γ
+    {{ fun _ t s' =>
+         exists C S', 
+           fresh S' (fst s') /\
+           let '(xs', f) := t in
+           project_vars Scope Funs (subst FVmap) Γ FVs S xs xs' C S' /\
+           is_exp_ctx f C }}.
+  Proof.
+    intros Hb Hfv. eapply pre_post_mp_l.
+    revert S Hb Hfv. induction xs; intros S Hb Hfv. 
+    - eapply return_triple. intros [x' d'] _ Hf.
+      eexists Hole_c. repeat eexists; eauto.
+      constructor.
+    - eapply pre_post_mp_r. eapply bind_triple.
+      + eapply get_var_project_var_sound; eauto.
+        intros x Hin. eapply Hb. 
+        inv Hin. constructor. eauto.
+      + intros [[x tau] f] [x' d']. eapply pre_eq_state.
+        intros [x'' d''] [C [S' [Hf [Hproj Hctx]]]].
+        eapply pre_post_mp_l. eapply bind_triple.
+        eapply (IHxs S'); eauto.
+        intros y Hin. eapply Hb. 
+        constructor 2. eassumption.
+        intros [xs' f'] [x''' d''']. eapply return_triple. 
+        intros [x'''' d''''] Hyp Heq'. inversion Heq'.
+        destruct Hyp as [C' [S'' [Hf' [Hproj' Hctx']]]]; eauto.
+        now rewrite <- H0; eauto.
+        exists (comp_ctx_f C C'), S''.
+        split; [ eassumption |].
+        split. now econstructor; eauto.
+        intros e. rewrite <- app_ctx_f_fuse. congruence.
+  Qed.
+  
+  (** Spec for [get_vars_with_types] *)
+  Lemma get_vars_with_types_project_vars_sound Scope Funs Γ FVs FVmap S xs :
+    binding_in_map (FromList xs) FVmap ->
+    FVmap_inv FVmap Scope Funs FVs ->
+    {{ fun s => fresh S (fst s) }}
+      get_vars_with_types utag xs FVmap Γ
+    {{ fun _ t s' =>
+         exists C S', 
+           fresh S' (fst s') /\
+           let '(xs', _, f) := t in
+           project_vars Scope Funs (subst FVmap) Γ FVs S xs xs' C S' /\
+           is_exp_ctx f C }}.
+  Proof.
+    intros Hb Hfv. eapply pre_post_mp_l.
+    revert S Hb Hfv. induction xs; intros S Hb Hfv. 
+    - eapply return_triple. intros [x' d'] _ Hf.
+      eexists Hole_c. repeat eexists; eauto. constructor.
+    - eapply pre_post_mp_r. eapply bind_triple.
+      + eapply get_var_project_var_sound; eauto.
+        intros x Hin. eapply Hb. 
+        inv Hin. constructor. eauto.
+      + intros [[x tau] f] [x' d']. eapply pre_eq_state.
+        intros [x'' d''] [C [S' [Hf [Hproj Hctx]]]].
+        eapply pre_post_mp_l. eapply bind_triple.
+        eapply (IHxs S'); eauto.
+        intros y Hin. eapply Hb. 
+        constructor 2. eassumption.
+        intros [[xs' ts'] f'] [x''' d''']. eapply return_triple. 
+        intros [x'''' d''''] Hyp Heq. inversion Heq.
+        destruct Hyp as [C' [S'' [Hf' [Hproj' Hctx']]]]; eauto.
+        now rewrite <- H0; eauto.
+        exists (comp_ctx_f C C'), S''.
+        split; [ eassumption |].
+        split. now econstructor; eauto.
+        intros e. rewrite <- app_ctx_f_fuse. congruence.
+  Qed.
+
+  Lemma subst_BoundVar_f_eq_subdomain FVmap x t S :
+    f_eq_subdomain S ((subst FVmap) {x ~> x}) (subst (M.set x (BoundVar t) FVmap)).
+  Proof.  
+    intros x'. unfold subst, extend. rewrite M.gsspec.
+    destruct (Coqlib.peq x' x). now eauto.
+    reflexivity. 
+  Qed.
+
+  Lemma subst_BoundVar_f_eq FVmap x t :
+    f_eq ((subst FVmap) {x ~> x}) (subst (M.set x (BoundVar t) FVmap)).
+  Proof.  
+    intros x'. unfold subst, extend. rewrite M.gsspec.
+    destruct (Coqlib.peq x' x). now eauto.
+    reflexivity. 
+  Qed.
+
+
+  Definition new_function_names FVmap : Ensemble var :=
+    fun x => exists y t1 t2, M.get y FVmap = Some (MRFun x t1 t2).
+
+  Lemma not_In_new_function_names_injective FVmap f:
+    ~ In _ (new_function_names FVmap) f ->
+    injective (subst FVmap) ->
+    injective ((subst FVmap) {f ~> f}).
+  Proof.
+    intros Hc Hinj x x' Heq. unfold extend in *.
+    destruct (Coqlib.peq x x'); eauto.
+    destruct (Coqlib.peq x f); eauto.
+    - destruct (Coqlib.peq x' f); try congruence.
+      exfalso. eapply Hc. 
+      eexists x'. unfold subst in Heq.
+      destruct (M.get x' FVmap) eqn:Heq'; eauto; try congruence.
+      subst. destruct v; try congruence.
+      eauto.
+    - destruct (Coqlib.peq x' f); [| now eauto ].
+      exfalso. eapply Hc. 
+      eexists x. unfold subst in Heq.
+      destruct (M.get x FVmap) eqn:Heq'; eauto; try congruence.
+      subst. destruct v; try congruence.
+      eauto.
+  Qed.
+
+  Lemma Disjoint_free_set FVmap Scope Funs FVs S :
+    binding_not_in_map S FVmap ->
+    FVmap_inv FVmap Scope Funs FVs ->
+    Disjoint _ S (Union var Scope
+                        (Union var Funs (FromList FVs))).
+  Proof.             
+    intros Hb [Hinv1 [Hinv2 Hinv3]].
+    constructor. intros x Hc. inv Hc. 
+    assert (Hdec1 : Decidable Scope).
+    { eapply Decidable_Same_set.
+      apply Same_set_sym. eassumption.
+      constructor. intros x'. destruct (M.get x' FVmap).
+      - destruct v; eauto;
+        right; intros [t' Hc]; congruence. 
+      - right. intros [t' Hc]. congruence. }
+    assert (Hdec2 : Decidable (Setminus _ Funs Scope)).
+    { eapply Decidable_Same_set.
+      apply Same_set_sym. eassumption.
+      constructor. intros x'. destruct (M.get x' FVmap).
+      - destruct v; eauto;
+        right; intros [y [t' [t'' Hc]]]; congruence. 
+      - right. intros [y [t' [t'' Hc]]]; congruence. }
+    destruct Hdec1, Hdec2.
+    destruct (Dec x). 
+    - eapply Hinv1 in H1. destruct H1 as [t Heq].
+      rewrite Hb in Heq; eauto. congruence.
+    - destruct (Dec0 x).
+      + eapply Hinv2 in H2. destruct H2 as [y [t [t' Heq]]].
+        rewrite Hb in Heq; eauto. congruence.
+      + inv H0; try contradiction.
+        inv H3. eapply H2; constructor; eauto.
+        unfold In, FromList in H0.        
+        edestruct In_nthN as [N Hnth]; [ eassumption |].
+        edestruct Hinv3 as [[t H'] _].
+        repeat split; eauto. intros Hin. eapply H2; constructor; eauto.
+        rewrite Hb in H'; eauto. congruence.
+  Qed.
+  
+  Lemma binding_not_in_map_antimon (A : Type) (S S' : Ensemble M.elt) (rho : M.t A):
+    Included M.elt S' S -> binding_not_in_map S rho -> binding_not_in_map S' rho.
+  Proof. 
+    intros Hin Hb x Hin'. eauto.
+  Qed.
+
+  Lemma binding_not_in_map_set_not_In_S {A} S map x (v : A) :
+    binding_not_in_map S map ->
+    ~ In _ S x ->
+    binding_not_in_map S (M.set x v map). 
+  Proof. 
+    intros HB Hnin x' Hin.
+    rewrite M.gsspec. destruct (Coqlib.peq x' x); subst; try contradiction. 
+    eauto. 
+  Qed.
+
+  Lemma new_function_names_set_BoundVar FVmap x t :
+    Included _ (new_function_names (M.set x (BoundVar t) FVmap)) (new_function_names FVmap).
+  Proof.
+    unfold new_function_names. intros x' [y [t' [t'' Hin]]].
+    rewrite M.gsspec in Hin. destruct (Coqlib.peq y x); try congruence.  
+    eauto.
+  Qed.
+
+  Import MonadNotation.
+
+  Transparent bind ret.
+
+  (** This identity is very useful to make the computation of the IH to appear
+      as a subcomputation in the goal *)
+  Lemma st_eq_Ecase {S} m1 (m2 : state S (var * type * (exp -> exp))) y :
+    st_eq
+      (ys <- m1 ;; 
+       ys' <- ret (y :: ys) ;;
+       t1 <- m2 ;;
+       let '(x, _ , f) := t1 in
+       ret (Ecase x ys', f))
+      (fe <- (ys <- m1 ;;
+             t1 <- m2 ;;
+             let '(x, _, f1) := t1 in    
+             ret (Ecase x ys, f1)) ;;
+       match fe with
+         | (Ecase x ys, f) =>
+           ret (Ecase x (y :: ys), f)
+         | _ => ret fe
+       end).
+  Proof.
+    unfold pbind, ret.
+    intros s. simpl. destruct (runState m1 s).
+    destruct (runState m2 s0). destruct p as [[x tau] f].
+    reflexivity.
+  Qed.
+
+  Opaque bind ret.
+
+  Lemma get_typeinfo_preserves_prop tau P :
+    {{ fun s => P (fst s) }} get_typeinfo tau {{ fun _ _ s => P (fst s) }}.
+  Proof.
+    eapply pre_post_mp_l. eapply bind_triple. eapply get_triple.
+    intros [x t] [x' t'].
+    destruct (TDict.get tau t); eapply return_triple;
+    intros [x'' t''] H HP; inv H; inv H0; inv H1; eauto.
+  Qed.
+
+  Lemma set_typeinfo_preserves_prop t P :
+    {{ fun s => P (fst s) }} set_typeinfo t {{ fun _ _ s => P (fst s) }}.
+  Proof.
+    eapply pre_post_mp_l. eapply bind_triple. eapply get_triple.
+    intros [x d] [x' d'].
+    destruct (TDict.hash t d).
+    eapply pre_post_mp_l. eapply bind_triple. eapply put_triple.
+    intros u [x'' d'']. eapply return_triple.
+    intros [x''' t'''] H1 [H2 H3] HP; inv H1; inv H2; inv H3; eauto.
+  Qed.
+  
+  Instance FVmap_inv_Scope_Proper :
+    Proper (Logic.eq ==> Same_set var ==> Logic.eq ==> Logic.eq ==> iff) FVmap_inv.
+  Proof. 
+    intros M1 M2 Heq1 S1 S2 Heq2 S3 S4 Heq3 l1 l2 Heq4; subst; split; intros [H1 [H2 H3]].
+    - (split; [| split ]); try rewrite <- Heq2; eauto. 
+      split. intros [Hnth [Hnin1 Hnin2]]. eapply H3. repeat split; eauto.
+      now rewrite Heq2.
+      intros H. rewrite <- Heq2. eapply H3. eassumption. 
+    - (split; [| split ]); try rewrite Heq2; eauto. 
+      split. intros [Hnth [Hnin1 Hnin2]]. eapply H3. repeat split; eauto.
+      now rewrite <- Heq2.
+      intros H. rewrite Heq2. eapply H3. eassumption. 
+  Qed.
+
+  Instance FVmap_inv_Funs_Proper :
+    Proper (Logic.eq ==> Logic.eq ==> Same_set var ==> Logic.eq ==> iff) FVmap_inv.
+  Proof. 
+    intros M1 M2 Heq1 S1 S2 Heq2 S3 S4 Heq3 l1 l2 Heq4; subst; split; intros [H1 [H2 H3]].
+    - (split; [| split ]); try rewrite <- Heq3; eauto.
+      split. intros [Hnth [Hnin1 Hnin2]]. eapply H3. repeat split; eauto.
+      now rewrite Heq3.
+      intros H. rewrite <- Heq3. eapply H3. eassumption. 
+    - (split; [| split ]); try rewrite Heq3; eauto. 
+      split. intros [Hnth [Hnin1 Hnin2]]. eapply H3. repeat split; eauto.
+      now rewrite <- Heq3.
+      intros H. rewrite Heq3. eapply H3. eassumption. 
+  Qed.
+
+  Lemma FVmapInv_add_params FVmap xs ts Scope Funs FVs :
+    FVmap_inv FVmap Scope Funs FVs ->
+    FVmap_inv (add_params xs ts FVmap) (Union _ Scope (FromList xs)) Funs FVs. 
+  Proof. 
+    revert FVmap ts Scope. induction xs; intros FVmap ts Scope Hinv.
+    - rewrite FromList_nil, Union_Empty_set_l. eauto.
+    - rewrite FromList_cons.
+      rewrite Union_assoc; rewrite Union_sym with (s2 := Singleton M.elt a), <- Union_assoc. 
+      destruct ts; eapply FVmap_inv_set_bound; eauto.
+  Qed.
+
+  Lemma binding_in_map_add_params S FVmap xs ts :
+    binding_in_map S FVmap ->
+    binding_in_map (Union _ S  (FromList xs)) (add_params xs ts FVmap).
+  Proof.
+    revert S FVmap ts. induction xs; intros S FVmap ts Hb.
+    - intros x. rewrite FromList_nil, Union_Empty_set_l. eauto.
+    - intros x. rewrite FromList_cons.
+      rewrite Union_sym with (s2 := FromList xs), Union_assoc.
+      simpl. destruct ts; eapply binding_in_map_set; eauto. 
+  Qed.
+
+  Lemma binding_not_in_map_add_params S FVmap xs ts :
+    binding_not_in_map S FVmap ->
+    Disjoint _ S (FromList xs) ->
+    binding_not_in_map S (add_params xs ts FVmap).
+  Proof.
+    revert S FVmap ts. induction xs; intros S FVmap ts Hb Hd.
+    - eauto.
+    - rewrite FromList_cons in Hd.
+      destruct ts; simpl; eapply binding_not_in_map_set_not_In_S; eauto.
+      + eapply IHxs. eassumption.
+        constructor. intros x Hc. inv Hc. eapply Hd. now constructor; eauto.
+      + intros Hc. eapply Hd. eauto.
+      + eapply IHxs. eassumption.
+        constructor. intros x Hc. inv Hc. eapply Hd. now constructor; eauto.
+      + intros Hc. eapply Hd. eauto.
+  Qed.
+
+  Lemma new_function_names_add_params FVmap xs ts :
+    Included  _ (new_function_names (add_params xs ts FVmap)) (new_function_names FVmap).
+  Proof.
+    revert FVmap ts. induction xs; intros FVmap ts; simpl. 
+    - apply Included_refl.
+    - destruct ts;
+      (eapply Included_trans;
+       [ eapply new_function_names_set_BoundVar | eapply IHxs ]).
+  Qed.
+
+  (* Lemma injective_add_params FVmap xs ts : *)
+  (*   Disjoint _ (new_function_names FVmap) (FromList xs) ->  *)
+  (*   injective (subst FVmap) -> *)
+  (*   injective (subst (add_params xs ts FVmap)). *)
+  (* Proof.  *)
+  (*   revert FVmap ts. induction xs; intros FVmap ts Hd Hinj. *)
+  (*   - eassumption.  *)
+  (*   - simpl. destruct ts; rewrite <- subst_BoundVar_f_eq; *)
+  (*     eapply not_In_new_function_names_injective. *)
+  (*     + intros Hc. eapply Hd. constructor. *)
+  (*       eapply new_function_names_add_params. eassumption.  *)
+  (*       rewrite FromList_cons. eauto. *)
+  (*     + eapply IHxs. constructor. intros x Hin.  *)
+  (*       inv Hin. eapply Hd. constructor; eauto. *)
+  (*       rewrite FromList_cons. eauto. *)
+  (*       eassumption. *)
+  (*     + intros Hc. eapply Hd. constructor. *)
+  (*       eapply new_function_names_add_params. eassumption.  *)
+  (*       rewrite FromList_cons. eauto. *)
+  (*     + eapply IHxs. constructor. intros x Hin.  *)
+  (*       inv Hin. eapply Hd. constructor; eauto. *)
+  (*       rewrite FromList_cons. eauto. *)
+  (*       eassumption. *)
+  (* Qed. *)
+
+  (* Lemma construct_lst_injection_add_params FVmap xs ts : *)
+  (*   Disjoint _ (new_function_names FVmap) (FromList xs) -> *)
+  (*   injective (subst FVmap) -> *)
+  (*   exists f, *)
+  (*     f_eq f (subst (add_params xs ts FVmap)) /\ *)
+  (*     construct_lst_injection (subst FVmap) xs xs f. *)
+  (* Proof. *)
+  (*   revert FVmap ts. induction xs; intros FVmap ts Hd Hinj.   *)
+  (*   - eexists. split. simpl. reflexivity. constructor. *)
+  (*   - assert (Hinj' : injective (subst (add_params (a :: xs) ts FVmap))). *)
+  (*     { apply injective_add_params; eauto. } *)
+  (*     rewrite FromList_cons in Hd. *)
+  (*     destruct ts; edestruct IHxs as [f [Heq Hinj'']].  *)
+  (*     + eapply Disjoint_Included_r; [ | eassumption ]. *)
+  (*       now apply Included_Union_r.  *)
+  (*     + eassumption. *)
+  (*     + eexists (f {a ~> a}). split.  *)
+  (*       simpl. rewrite Heq. eapply subst_BoundVar_f_eq. *)
+  (*       constructor. eassumption.  *)
+  (*       rewrite Heq. simpl in Hinj'. rewrite subst_BoundVar_f_eq. *)
+  (*       eassumption. *)
+  (*     + eapply Disjoint_Included_r; [ | eassumption ]. *)
+  (*       now apply Included_Union_r.  *)
+  (*     + eassumption. *)
+  (*     + eexists (f {a ~> a}). split.  *)
+  (*       simpl. rewrite Heq. eapply subst_BoundVar_f_eq. *)
+  (*       constructor. eassumption.  *)
+  (*       rewrite Heq. simpl in Hinj'. rewrite subst_BoundVar_f_eq. *)
+  (*       eassumption. *)
+  (* Qed. *)
+          
+  Lemma FVmap_inv_empty :
+    FVmap_inv (Maps.PTree.empty VarInfo) (Empty_set M.elt) (Empty_set M.elt) [].
+  Proof.
+    repeat split; (try now intros Hc; inv Hc); (try now intros x Hc; inv Hc). 
+    intros x Hx. destruct Hx as [t Hget]. rewrite M.gempty in Hget. now inv Hget.
+    destruct H as [x' [t [t' Hget]]]. rewrite M.gempty in Hget. now inv Hget.
+    destruct H as [t Hget]. rewrite M.gempty in Hget. now inv Hget.
+  Qed.
+  
+  Lemma nthN_app {A} (l1 l2 : list A) N :
+    (nthN (l1 ++ l2) N = nthN l1 N) \/
+    (nthN (l1 ++ l2) N = nthN l2 (N - N.of_nat (length l1))%N /\ (N.of_nat (length l1) <= N)%N).
+  Proof. 
+    revert N; induction l1; intros N.
+    - right. rewrite app_nil_l, N.sub_0_r. split; eauto. simpl. zify; omega.
+    - destruct N; [now eauto |].
+      destruct (IHl1 ((N.pos p)-1)%N) as [H1 | [H2 H3]].
+      now eauto.
+      replace (N.of_nat (length (a :: l1))) with (1 + N.of_nat (length l1))%N.
+      replace (N.pos p - (1 + N.of_nat (length l1)))%N with
+      (N.pos p - 1 - N.of_nat (length l1))%N.
+      right. split. now eauto. zify. omega. 
+      zify; omega. 
+      simpl (length _). rewrite Nnat.Nat2N.inj_succ.
+      zify. omega. 
+  Qed.
+  
+  Lemma nthN_is_Some_length {A} (l : list A) N x :
+    nthN l N = Some x ->
+    (N < N.of_nat (length l))%N.
+  Proof. 
+    revert N. induction l; intros N Heq.
+    - inv Heq. 
+    - destruct N. inv Heq.
+      unfold length. rewrite Nnat.Nat2N.inj_succ. zify. omega. 
+      assert (Hlt : ((N.pos p)-1 < N.of_nat (length l))%N) by eauto.
+      simpl (length _). rewrite Nnat.Nat2N.inj_succ.
+      zify. omega. 
+  Qed.
+  
+  Lemma nthN_app_geq {A} (l1 l2 : list A) N :
+    (N.of_nat (length l1) <= N)%N ->
+    nthN (l1 ++ l2) N = nthN l2 (N - N.of_nat (length l1))%N.
+  Proof.
+    revert N. induction l1; intros N Heq.
+    - simpl. rewrite N.sub_0_r. reflexivity.
+    - simpl length in *. 
+      destruct N. 
+      zify. omega.
+      rewrite Nnat.Nat2N.inj_succ.
+      rewrite <- N.add_1_l, N_as_DT.sub_add_distr. 
+      rewrite <- IHl1.
+      reflexivity. zify. omega. 
+  Qed.
+  
+  Lemma nthN_is_Some_app {A} (l1 l2 : list A) N x :
+    nthN l1 N = Some x ->
+    nthN (l1 ++ l2) N = Some x.
+  Proof.
+    revert N. induction l1; intros N Heq.
+    - inv Heq.
+    - destruct N. inv Heq. reflexivity.
+      simpl. eauto.
+  Qed.
+  
+  Lemma FVmap_inv_set_free_var FVmap Scope Funs FVs x n t:
+    FVmap_inv FVmap Scope Funs FVs ->
+    N.of_nat (length FVs) = n ->
+    ~ In _ Scope x -> ~ In  _ Funs x -> ~ List.In x FVs ->
+    FVmap_inv (Maps.PTree.set x (FVar n t) FVmap) Scope Funs (FVs ++ [x]). 
+  Proof.  
+    intros [H1 [H2 H3]] Hlen Hnin1 Hnin2.
+    split; [| split ]. 
+    - split.
+      + intros x' Hin. assert (Hin' := Hin).
+        eapply H1 in Hin. edestruct Hin as [t' Heq].
+        destruct (Coqlib.peq x' x).
+        subst; contradiction.
+        eexists. rewrite M.gso; eauto.
+      + intros x' [t' Hget]. eapply H1. 
+        rewrite M.gsspec in Hget. destruct (Coqlib.peq x' x).
+        subst; congruence.
+        now eauto.
+    - split.
+      + intros x' Hin. assert (Hin' := Hin). inv Hin'. 
+        eapply H2 in Hin. edestruct Hin as [y [t1 [t2 Heq]]].
+        destruct (Coqlib.peq x' x).
+        subst; contradiction.
+        eexists. rewrite M.gso; eauto.
+      + intros x' [y [t1 [t2 Hget]]]. eapply H2. 
+        rewrite M.gsspec in Hget. destruct (Coqlib.peq x' x).
+        subst; congruence.
+        now eauto.
+    - intros N x'. split.
+      + intros [Hnth [Hnin1' Hnin2']].
+        destruct (nthN_app FVs [x] N) as [Hn | [Hn Hlen']].
+        * destruct (Coqlib.peq x' x); subst.
+          exfalso. eapply H. eapply nthN_In. rewrite <- Hnth. now eauto.
+          edestruct H3 as [[t' Hget] _].
+          repeat split; eauto. rewrite <- Hnth. now eauto.
+          eexists. now rewrite M.gso; eauto.
+        * subst. rewrite Hnth in Hn. eapply nthN_is_Some_length in Hnth.
+          rewrite app_length in Hnth. simpl length in *.
+          destruct (N - N.of_nat (length FVs))%N eqn:Heq; simpl in Hn; try congruence.
+          inv Hn. eexists. rewrite M.gss; eauto.
+          repeat f_equal. zify. omega. 
+      + subst. intros [t' Hget].
+        rewrite M.gsspec in Hget. destruct (Coqlib.peq x' x).
+        * subst. inv Hget. repeat split; eauto.
+          rewrite nthN_app_geq. rewrite N.sub_diag. reflexivity. 
+          zify; omega. 
+        * edestruct H3 as [_ [H1' [H2' H3']]].
+          now eexists; eauto.
+          repeat split; eauto. apply nthN_is_Some_app. eassumption.
+  Qed.
+
+  Lemma FromList_app {A} (l1 l2 : list A) :
+    Same_set _ (FromList (l1 ++ l2)) (Union _ (FromList l1) (FromList l2)). 
+  Proof.
+    induction l1. 
+    - rewrite FromList_nil, Union_Empty_set_r. now apply Same_set_refl.
+    - rewrite FromList_cons, <- Union_assoc, <- IHl1, <- FromList_cons, app_comm_cons. 
+      now apply Same_set_refl.
+  Qed.
+
+  Lemma Complement_antimon {A} S1 S2 :
+    Included A S1 S2 ->
+    Included A (Complement _ S2) (Complement _ S1).
+  Proof.
+    intros Hin x Hin' y. eauto.
+  Qed.
+  
+  Lemma make_env_spec fv FVmap_o Γ_n Γ_o Scope Funs FVs S :
+    binding_in_map (FromList (PS.elements fv)) FVmap_o ->
+    binding_not_in_map (Union M.elt S (Singleton M.elt Γ_o)) FVmap_o ->
+    FVmap_inv FVmap_o Scope Funs FVs ->
+    {{ fun s => fresh S (fst s) }}
+      make_env utag env_tag fv (Maps.PTree.empty VarInfo) FVmap_o Γ_n Γ_o 
+    {{ fun s t  s' =>
+         let '(_, FVmap_n, f) := t in
+         exists C S' FVs' tau t,
+           fresh S' (fst s') /\
+           project_vars Scope Funs (subst FVmap_o) Γ_o FVs S (PS.elements fv) FVs' C S' /\
+           is_exp_ctx f (comp_ctx_f C (Econstr_c Γ_n tau t FVs' Hole_c)) /\
+           binding_in_map (FromList (PS.elements fv)) FVmap_n /\
+           binding_not_in_map (Complement _ (FromList (PS.elements fv))) FVmap_n /\
+           FVmap_inv FVmap_n (Empty_set _) (Empty_set _) (PS.elements fv)
+     }}.
+  Proof.
+    intros Hb1 Hb2 Minv. eapply bind_triple. 
+    - eapply get_vars_with_types_project_vars_sound; eauto.
+    - intros [[xs ts] f] s1.
+      eapply pre_existential. intros C1. eapply pre_existential. intros S'.
+      eapply pre_uncurry_r. intros [Hvars Hctx].
+      eapply bind_triple. now eapply set_typeinfo_preserves_prop.
+      intros tau s2. eapply return_triple.
+      intros s3 Hf. do 6 eexists. eassumption. 
+      repeat (split; [ eassumption |]). split.
+      + intros e. rewrite Hctx. rewrite <- app_ctx_f_fuse.
+        f_equal. reflexivity.
+      + clear. 
+        assert (He : FVmap_inv (Maps.PTree.empty VarInfo)
+                               (Empty_set M.elt) (Empty_set M.elt) (@nil PS.elt))
+          by apply FVmap_inv_empty.
+        assert (Hb : binding_in_map (FromList (@nil PS.elt)) (Maps.PTree.empty VarInfo))
+          by (intros x H; inv H).
+        assert (Hb' : binding_not_in_map (Complement _ (FromList ((@nil PS.elt))))
+                                         (Maps.PTree.empty VarInfo))
+          by (intros x H; rewrite Maps.PTree.gempty; reflexivity).
+        assert (Hlen : N.of_nat (@length PS.elt []) = 0%N) by eauto.
+        assert (Hnin : forall x, List.In x (PS.elements fv) -> ~ List.In x (@nil PS.elt))
+          by (intros x H1 H2; inv H2).
+        assert (Hdup :  NoDupA eq (PS.elements fv)) by apply PS.elements_spec2w.
+        replace (PS.elements fv) with ([] ++ PS.elements fv) at 1 3 6 by reflexivity.
+        revert Hlen He Hb Hb' Hnin Hdup. generalize (Maps.PTree.empty VarInfo) as FVmap_i.
+        generalize (@nil PS.elt). generalize 0%N. 
+        induction (PS.elements fv); intros n vars FVmap_i Hlen Hinv Hb Hb' Hnin Hdup.
+        * simpl. rewrite app_nil_r. simpl. eauto.
+        * simpl. replace (vars ++ a :: l) with ((vars ++ [a]) ++ l). simpl.
+          eapply IHl. rewrite app_length. simpl. zify. omega.
+          eapply FVmap_inv_set_free_var. now eauto. eassumption. 
+          now intros Hc; inv Hc. now intros Hc; inv Hc. 
+          eapply Hnin. constructor. reflexivity.
+          intros x H. eapply binding_in_map_set. eassumption.
+          rewrite FromList_app, FromList_cons, FromList_nil, Union_Empty_set_l in H.
+          eassumption.
+          eapply binding_not_in_map_set_not_In_S.
+          eapply binding_not_in_map_antimon; [| eassumption ]. 
+          eapply Complement_antimon. rewrite FromList_app. now apply Included_Union_l.
+          intros Hc. eapply Hc. rewrite FromList_app, FromList_cons, FromList_nil. now eauto.
+          intros x Hin Hc. eapply Hnin.
+          now constructor 2; eauto. inv Hdup.
+          apply Coqlib.in_app in Hc. inv Hc; eauto. inv H. 
+          exfalso. eapply H1. eapply In_InA. eauto. now eapply Pos.eq_equiv. 
+          eassumption. now inv H0. now inv Hdup.
+          rewrite <- app_assoc. reflexivity.
+  Qed.
+
+  Lemma subst_MRFun_f_eq (FVmap : VarInfoMap) (x x' : var) (t t': type) :
+    f_eq ((subst FVmap) {x ~> x'}) (subst (M.set x (MRFun x' t t') FVmap)).
+  Proof.
+    unfold subst. intros y. unfold extend.
+    rewrite M.gsspec. destruct (Coqlib.peq y x); eauto.
+  Qed.
+
+  Instance image_Proper {A B} : Proper (f_eq ==> Logic.eq ==> Same_set _) (@image A B).
+  Proof.
+    intros x1 x2 Heq s1 s2 Heq'; subst.
+    split; intros x [y1 [Hin Heq']]; subst;
+    eexists; eauto.
+  Qed.
+
+  Instance f_eq_subdomain_Proper_Same_set {A B} :
+    Proper (Same_set A ==> eq ==> eq ==> iff) (@f_eq_subdomain A B).
+  Proof.
+    intros S1 S2 Hseq f1 f1' Heq1 f2 f2' Heq2; subst; split; intros Hfeq x HS;
+    apply Hfeq; eapply Hseq; eassumption.
+  Qed.
+
+  Instance f_eq_subdomain_Proper_f_eq_l {A B} :
+    Proper (eq ==> f_eq ==> eq ==> iff) (@f_eq_subdomain A B).
+  Proof.
+    intros S1 S2 Heq f1 f1' Heq1 f2 f2' Heq2; subst; split; intros Hfeq x HS.
+    now rewrite <- Heq1; eauto. now rewrite Heq1; eauto.
+  Qed.
+
+  Instance f_eq_subdomain_Proper_f_eq_r {A B} :
+    Proper (eq ==> eq ==> f_eq ==> iff) (@f_eq_subdomain A B).
+  Proof.
+    intros S1 S2 Heq f1 f1' Heq1 f2 f2' Heq2; subst; split; intros Hfeq x HS.
+    now rewrite <- Heq2; eauto. now rewrite Heq2; eauto.
+  Qed.
+
+  Lemma f_eq_subdomain_extend S (f f' : var -> var) x y :
+    f_eq_subdomain S f f' ->
+    f_eq_subdomain (Union _ (Singleton _ x) S) (f{x ~> y}) (f'{x ~> y}).
+  Proof. 
+    intros Heq. 
+    unfold extend. intros z Hin. 
+    destruct (Coqlib.peq z x). now eauto.
+    apply Heq. inv Hin; [| now eauto ]. inv H; congruence. 
+  Qed.
+  
+  Lemma f_eq_subdomain_antimon {A B} S S' (f f' : A -> B) :
+    Included _ S' S ->
+    f_eq_subdomain S f f' ->
+    f_eq_subdomain S' f f'.
+  Proof.
+    intros Hinc Hfeq x Hin; eauto.
+  Qed.
+
+  Lemma f_eq_subdomain_extend_not_In_S_l f1 S f2 x x'  : 
+    ~ In _ S x ->
+    f_eq_subdomain S f1 f2 ->
+    f_eq_subdomain S (f1{x~>x'}) f2.
+  Proof.
+    intros Hin Hfeq y HIn.
+    rewrite extend_gso. now eauto.
+    intros Hc. subst. contradiction.
+  Qed.
+
+  Lemma f_eq_subdomain_extend_not_In_S_r f1 S f2 x x'  : 
+    ~ In _ S x ->
+    f_eq_subdomain S f1 f2 ->
+    f_eq_subdomain S f1 (f2{x~>x'}).
+  Proof.
+    intros Hin Hfeq y HIn.
+    rewrite extend_gso. now eauto.
+    intros Hc. subst. contradiction.
+  Qed.
+
+
+  Lemma make_full_closure_spec B FVmap_n FVmap_o Γ Scope Funs FVs FVs' typ S S1 S2 S1' S2' :
+    binding_in_map S1 FVmap_o -> 
+    binding_in_map S2 FVmap_n ->
+    binding_not_in_map S1' FVmap_o -> 
+    binding_not_in_map S2' FVmap_n ->
+    FVmap_inv FVmap_o Scope Funs FVs ->
+    FVmap_inv FVmap_n (Empty_set _) (Empty_set _) FVs' ->
+    {{ fun s => fresh S (fst s) }}
+      make_full_closure utag tag_bij unknown_type B FVmap_n FVmap_o Γ typ
+    {{ fun s t s' =>
+         let '(FVmap_n', FVmap_o', f) := t in
+         exists C S',
+           fresh S' (fst s') /\
+           make_closures B S Γ C (subst FVmap_n') S' /\
+           is_exp_ctx f C /\
+           f_eq_subdomain (Setminus _ Funs (Union _ Scope (name_in_fundefs B)))
+                          (subst FVmap_o) (subst FVmap_o') /\
+           binding_in_map (Union _ S1 (name_in_fundefs B)) FVmap_o' /\
+           binding_in_map (Union _ S2 (name_in_fundefs B)) FVmap_n' /\
+           binding_not_in_map (Setminus _ S1' (name_in_fundefs B)) FVmap_o' /\
+           binding_not_in_map (Setminus _ S2' (name_in_fundefs B)) FVmap_n' /\
+           FVmap_inv FVmap_o' (Union _ (name_in_fundefs B) Scope) Funs FVs /\
+           FVmap_inv FVmap_n' (Empty_set _) (name_in_fundefs B) FVs'
+     }}.
+  Proof.
+    revert FVmap_n FVmap_o Γ Scope Funs FVs FVs' typ S S1 S2 S1' S2'.
+    induction B;
+      intros FVmap_n FVmap_o Γ Scope Funs FVs FVs' typ S
+             S1 S2 S1' S2' Hb1 Hb2 Hb1' Hb2'  Minv_o Minv_n. 
+    - eapply bind_triple; [ now apply get_name_fresh |].
+      intros x s1. eapply pre_uncurry_l. intros Hx.
+      eapply bind_triple; [ eapply IHB; eassumption |].
+      intros [[FVmap_n' FVmap_o'] f] _.
+      eapply pre_existential. intros C. eapply pre_existential. intros S'.
+      eapply pre_uncurry_r. intros [Hclo [Hctx [Hfeq [Hbn [Hbo [Hbn' [Hbo' [Minv_o' Minv_n']]]]]]]].
+      eapply bind_triple; [ now apply get_typeinfo_preserves_prop |].
+      intros t_inf s2.
+      eapply bind_triple with
+      (post' := fun _ _ s =>  fresh S' (fst s)).
+      + destruct t_inf; try now apply return_triple. 
+        eapply bind_triple. now apply set_typeinfo_preserves_prop.
+        intros. eapply bind_triple. now apply set_typeinfo_preserves_prop.
+        intros. now apply return_triple. 
+      + intros [typ' typ''] _. apply return_triple. 
+        intros s3 Hf. do 2 eexists.
+        split. eassumption. 
+        split. econstructor. eassumption. eapply Hx. zify; omega.
+        rewrite <- subst_MRFun_f_eq. reflexivity.
+        split. intros e'. simpl. rewrite Hctx. reflexivity.
+        split. rewrite <- subst_BoundVar_f_eq.
+        apply f_eq_subdomain_extend_not_In_S_r.
+        intros Hc. inv Hc. eapply H0. right. left. now eauto.
+        eapply f_eq_subdomain_antimon; [| eassumption ].
+        apply Included_Setminus_compat. now apply Included_refl.
+        apply Included_Union_compat. now apply Included_refl.
+        now apply Included_Union_r.
+        split. eapply binding_in_map_antimon; [| eapply binding_in_map_set; eassumption ].
+        simpl. rewrite (Union_sym (Singleton _ v)), Union_assoc. now apply Included_refl.
+        split.  eapply binding_in_map_antimon; [| eapply binding_in_map_set; eassumption ].
+        simpl. rewrite (Union_sym (Singleton _ v)), Union_assoc. now apply Included_refl.
+        split. eapply binding_not_in_map_set_not_In_S.
+        eapply binding_not_in_map_antimon; [| eassumption ]. 
+        apply Included_Setminus_compat. now apply Included_refl.
+        now apply Included_Union_r.
+        intros Hc. inv Hc. eapply H0. left. now eauto.
+        split. eapply binding_not_in_map_set_not_In_S.
+        eapply binding_not_in_map_antimon; [| eassumption ].
+        apply Included_Setminus_compat. now apply Included_refl.
+        now apply Included_Union_r.
+        intros Hc. inv Hc. eapply H0. left. now eauto.
+        split. simpl. rewrite <- Union_assoc. eapply FVmap_inv_set_bound.
+        eassumption.
+        simpl. apply FVmap_inv_set_funs. now apply not_In_Empty_set.
+        eassumption. 
+    - eapply return_triple. intros s Hs. do 2 eexists.
+      split. eassumption. split. now constructor.
+      split. intros e. reflexivity.
+      split. intros x H. reflexivity.
+      split. intros x H. eapply Hb1. now rewrite Union_Empty_set_l in H.
+      split. intros x H. eapply Hb2. now rewrite Union_Empty_set_l in H.
+      split. eapply binding_not_in_map_antimon; [| eassumption ].
+      now apply Subset_Setminus.
+      split. eapply binding_not_in_map_antimon; [| eassumption ].
+      now apply Subset_Setminus.
+      split. rewrite Union_Empty_set_r. eassumption.
+      eassumption. 
+  Qed.
+
+  Lemma image_extend_not_In f x x' S :
+    ~ In _ S x ->
+    Same_set _ (image (f {x ~> x'} ) S) (image f S).
+  Proof.    
+    intros Hnin.
+    split; intros y [y' [Hin Heq]]. rewrite extend_gso in Heq.
+    now eexists; eauto. intros Hc. subst. contradiction.
+    eexists; split; eauto. rewrite extend_gso. now eauto.
+    intros Hc. subst. contradiction.
+  Qed.
+
+  Instance equivalence_f_eq_subdomain {A B} S : Equivalence (@f_eq_subdomain A B S). 
+  Proof. 
+    constructor; try now constructor.
+    intros f1 f2 Heq x HS; rewrite Heq. reflexivity. eassumption.
+    intros f1 f2 f3 Heq1 Heq2 x HS; rewrite Heq1. now eauto. eassumption.
+  Qed.      
+
+  Lemma image_Setminus_extend f v v' S :
+    Included _ (image (f {v ~> v'}) (Setminus M.elt S  (Singleton var v)))
+             (image f S).
+  Proof.
+    intros x [y [Hin Heq]]; subst.
+    destruct (Coqlib.peq v y); subst.
+    - inv Hin. exfalso. eauto.
+    - rewrite extend_gso; [| now eauto ].
+      eexists; esplit; auto. inv Hin. now eauto.
+  Qed.
+
+  Instance project_var_Proper Scope Funs :
+    Proper
+      (f_eq_subdomain (Setminus _ Funs Scope) ==> eq ==> eq ==> eq ==> eq ==> eq ==> eq ==> eq ==> iff)
+      (project_var Scope Funs).
+  Proof. 
+    constructor; subst; intros Hproj; inv Hproj; try (now constructor; eauto).
+    - rewrite H; now econstructor; eauto.
+    - rewrite <- H; now econstructor; eauto.
+  Qed.
+  
+  Instance project_vars_Proper Scope Funs :
+    Proper
+      (f_eq_subdomain (Setminus _ Funs Scope) ==> eq ==> eq ==> eq ==> eq ==> eq ==> eq ==> eq ==> iff)
+      (project_vars Scope Funs).
+  Proof. 
+      constructor; subst; intros Hproj; induction Hproj; try (now constructor; eauto).
+      - econstructor. eapply project_var_Proper; eauto.
+        now symmetry. now eauto.
+      - econstructor. now eapply project_var_Proper; eauto. now eauto.
+  Qed.
+
+  Lemma image_f_eq_subdomain {A B} (f1 f2 : A -> B) S :
+    f_eq_subdomain S f1 f2 ->
+    Same_set _ (image f1 S) (image f2 S).
+  Proof.
+    intros Heq; split; intros x [y [Hin Heq']]; subst; 
+    (eexists; split; [ now eauto |]); now rewrite Heq.
+  Qed.
+
+  Lemma Closure_conversion_f_eq_subdomain_mut :
+    (forall e Scope Funs σ σ' FVs Γ e' C
+       (Hcc : Closure_conversion Scope Funs σ Γ FVs e e' C)
+       (Hfeq : f_eq_subdomain (Setminus _ Funs Scope) σ σ'),
+       Closure_conversion Scope Funs σ' Γ FVs e e' C) /\
+    (forall B Funs σ σ' FVs B'
+       (Hinc : Included _ (name_in_fundefs B) Funs)
+       (Hcc : Closure_conversion_fundefs Funs σ FVs B B')
+       (Hfeq : f_eq_subdomain Funs σ σ'),
+       Closure_conversion_fundefs Funs σ' FVs B B').
+  Proof. 
+    eapply exp_def_mutual_ind; intros; inv Hcc.
+    - econstructor; try reflexivity. rewrite <- image_f_eq_subdomain; [| eassumption ].
+      eassumption.
+      eapply project_vars_Proper; [ symmetry; eassumption | | | | | | | | ];
+      try reflexivity. eassumption.
+      eapply H. eassumption. eapply f_eq_subdomain_antimon; [| eassumption ].
+      apply Included_Setminus_compat. now apply Included_refl.
+      now apply Included_Union_r.
+    - econstructor; try reflexivity. rewrite <- image_f_eq_subdomain; [| eassumption ].
+      eassumption.
+      eapply project_var_Proper; [ symmetry; eassumption | | | | | | | | ];
+      try reflexivity. eassumption.
+      inv H10. constructor.
+    - econstructor; try reflexivity. rewrite <- image_f_eq_subdomain; [| eassumption ].
+      eassumption.
+      eapply project_var_Proper; [ symmetry; eassumption | | | | | | | | ];
+      try reflexivity. eassumption.
+      inv H12. inv H4. simpl in H1; subst. destruct H2 as [C' [e' [Heq Hcc]]].
+      constructor. now split; eauto.
+      assert (Hcc' : Closure_conversion Scope Funs σ' Γ FVs (Ecase v l)  (Ecase x' l') C).
+      { eapply H0. econstructor; eauto. eassumption. }
+      now inv Hcc'.
+    - econstructor; try reflexivity. rewrite <- image_f_eq_subdomain; [| eassumption ].
+      eassumption.
+      eapply project_var_Proper; [ symmetry; eassumption | | | | | | | | ];
+      try reflexivity. eassumption.
+      eapply H. eassumption. eapply f_eq_subdomain_antimon; [| eassumption ].
+      apply Included_Setminus_compat. now apply Included_refl.
+      now apply Included_Union_r.
+    - econstructor; try reflexivity. eassumption.
+      rewrite <- image_f_eq_subdomain; [| eassumption ].
+      eassumption.
+      eapply project_vars_Proper; [ symmetry; eassumption | | | | | | | | ];
+      try reflexivity. eassumption.
+      rewrite <- image_f_eq_subdomain; [| eassumption ].
+      eassumption. eassumption.
+      rewrite <- image_f_eq_subdomain; [| eassumption ].
+      eassumption. eassumption. eapply H.
+      now apply Included_refl. eassumption. reflexivity.
+      eapply H0. eassumption. eapply f_eq_subdomain_antimon; [| eassumption ].
+      apply Included_Setminus_compat. now apply Included_refl.
+      now apply Included_Union_r.
+    - econstructor; try reflexivity; try eassumption.
+      rewrite <- image_f_eq_subdomain; [| eassumption ].
+      eassumption.
+      eapply project_vars_Proper; [ symmetry; eassumption | | | | | | | | ];
+      try reflexivity. eassumption.
+    - econstructor; try reflexivity. rewrite <- image_f_eq_subdomain; [| eassumption ].
+      eassumption.
+      eapply project_vars_Proper; [ symmetry; eassumption | | | | | | | | ];
+      try reflexivity. eassumption.
+      eapply H. eassumption. eapply f_eq_subdomain_antimon; [| eassumption ].
+      apply Included_Setminus_compat. now apply Included_refl.
+      now apply Included_Union_r.
+    - rewrite Hfeq. econstructor; try eassumption.
+      rewrite <- image_f_eq_subdomain; [| eassumption ]. eassumption.
+      eapply H0; [| now eauto | now eauto ].
+      eapply Included_trans; [| eassumption ]. now apply Included_Union_r.
+      eapply H. eassumption.
+      eapply f_eq_subdomain_antimon; [| eassumption ].
+      now apply Subset_Setminus.
+      eapply Hinc. left. eauto.
+    - constructor. 
+  Qed.
+
+  Corollary Closure_conversion_f_eq_subdomain :
+    forall e Scope Funs σ σ' FVs Γ e' C
+       (Hcc : Closure_conversion Scope Funs σ Γ FVs e e' C)
+       (Hfeq : f_eq_subdomain (Setminus _ Funs Scope) σ σ'),
+      Closure_conversion Scope Funs σ' Γ FVs e e' C.
+  Proof.
+    now apply Closure_conversion_f_eq_subdomain_mut.
+  Qed.
+
+  Corollary Closure_conversion_fundefs_f_eq_subdomain :
+  (forall B Funs σ σ' FVs B'
+       (Hinc : Included _ (name_in_fundefs B) Funs)
+       (Hcc : Closure_conversion_fundefs Funs σ FVs B B')
+       (Hfeq : f_eq_subdomain Funs σ σ'),
+       Closure_conversion_fundefs Funs σ' FVs B B').
+  Proof. 
+    now apply Closure_conversion_f_eq_subdomain_mut.
+  Qed.
+
+
+  Lemma bound_var_occurs_free_Econstr_Included x tau t ys e :
+    Included _ (Union _ (bound_var e) (occurs_free e))
+             (Union _ (bound_var (Econstr x tau t ys e))
+                    (occurs_free (Econstr x tau t ys e))).
+  Proof.
+    rewrite bound_var_Econstr, <- Union_assoc.
+    apply Included_Union_compat. now apply Included_refl. 
+    eapply Included_trans. now apply occurs_free_Econstr_Included.
+    rewrite Union_sym. now apply Included_refl.
+  Qed.
+
+  Lemma bound_var_occurs_free_Ecase_Included c e x P:
+    List.In (c, e) P ->
+    Included _ (Union _ (bound_var e) (occurs_free e))
+             (Union _ (bound_var (Ecase x P))
+                    (occurs_free (Ecase x P))).
+  Proof.
+    intros Hin x' Hin'. inv Hin'.
+    now left; eauto.
+    right. eapply occurs_free_Ecase_Included; now eauto.
+  Qed.
+
+  Lemma bound_var_occurs_free_Ecase_cons_Included c e x P:
+    Included _ (Union _ (bound_var (Ecase x P))
+                      (occurs_free (Ecase x P)))
+             (Union _ (bound_var (Ecase x ((c, e) :: P)))
+                    (occurs_free (Ecase x ((c, e) :: P)))).
+  Proof.
+    rewrite bound_var_Ecase_cons, <- Union_assoc.
+    eapply Included_Union_mon_r.
+    apply Included_Union_compat. now apply Included_refl.
+    eapply Included_trans with (s2 := occurs_free (Ecase x ((c, e) :: P))).
+    intros y Hin. now apply Free_Ecase3. now apply Included_refl.
+  Qed.
+
+  Lemma bound_var_occurs_free_Eproj_Included x tau N y e :
+    Included _ (Union _ (bound_var e) (occurs_free e))
+             (Union _ (bound_var (Eproj x tau N y e))
+                    (occurs_free (Eproj x tau N y e))).
+  Proof.
+    rewrite bound_var_Eproj, <- Union_assoc.
+    apply Included_Union_compat. now apply Included_refl. 
+    eapply Included_trans. now apply occurs_free_Eproj_Included.
+    rewrite Union_sym. now apply Included_refl.
+  Qed.
+
+
+  Lemma bound_var_occurs_free_Efun_Included B e :
+    Included _ (Union _ (bound_var e) (occurs_free e))
+             (Union _ (bound_var (Efun B e))
+                    (occurs_free (Efun B e))).
+  Proof.
+    rewrite bound_var_Efun, (Union_sym _ (bound_var e)), <- Union_assoc.
+    apply Included_Union_compat. now apply Included_refl. 
+    eapply Included_trans. now apply occurs_free_Efun_Included.
+    rewrite Union_sym. apply Included_Union_compat.
+    now apply name_in_fundefs_bound_var_fundefs. now apply Included_refl.
+  Qed.
+
+  Lemma bound_var_occurs_free_fundefs_Efun_Included B e :
+    Included _ (Union _ (bound_var_fundefs B) (occurs_free_fundefs B))
+             (Union _ (bound_var (Efun B e))
+                    (occurs_free (Efun B e))).
+  Proof.
+    rewrite bound_var_Efun, (Union_sym _ (bound_var e)), <- Union_assoc.
+    apply Included_Union_mon_r.
+    apply Included_Union_compat. now apply Included_refl. 
+    rewrite occurs_free_Efun. now apply Included_Union_mon_l.
+  Qed.
+
+  Lemma bound_var_occurs_free_Eprim_Included x tau f ys e :
+    Included _ (Union _ (bound_var e) (occurs_free e))
+             (Union _ (bound_var (Eprim x tau f ys e))
+                    (occurs_free (Eprim x tau f ys e))).
+  Proof.
+    rewrite bound_var_Eprim, <- Union_assoc.
+    apply Included_Union_compat. now apply Included_refl. 
+    eapply Included_trans. now apply occurs_free_Eprim_Included.
+    rewrite Union_sym. now apply Included_refl.
+  Qed.
+
+  Lemma Included_Setminus_Disjoint {A} s1 s2 :
+    Disjoint _ s1 s2 ->
+    Same_set A s1 (Setminus _ s1 s2).
+  Proof.
+    intros Hd.
+    split; intros x H. constructor; eauto. intros Hc; eapply Hd; eauto. 
+    inv H; eauto.
+  Qed.
+
+  Corollary fundefs_fv_correct B :
+    Same_set var (occurs_free_fundefs B)
+             (FromList (PS.elements (fundefs_fv B (fundefs_names B)))).
+  Proof.
+    split; intros x H.
+    eapply exp_fv_fundefs_fv_correct in H. eapply PS.elements_spec1 in H.
+    eapply InA_alt in H. edestruct H as [y [Heq Hin]]. subst. eauto. 
+    eapply exp_fv_fundefs_fv_correct. eapply PS.elements_spec1.
+    eapply In_InA. now eapply PS.E.eq_equiv. eassumption.
+  Qed.
+
+  Lemma subst_add_params_f_eq_subdomain S l ts FVmap :
+    Disjoint _ (FromList l) S ->
+    f_eq_subdomain S
+     (subst (add_params l ts FVmap)) (subst FVmap).
+  Proof.
+    intros Hd.
+    revert ts; induction l; intros ts.
+    - simpl. reflexivity.
+    - simpl. destruct ts.
+      rewrite <- subst_BoundVar_f_eq_subdomain.
+      eapply f_eq_subdomain_extend_not_In_S_l.
+      intros H. eapply Hd. constructor. rewrite FromList_cons.
+      now left. eassumption.
+      eapply IHl. eapply Disjoint_Included_l; [| eassumption ].
+      rewrite FromList_cons. now apply Included_Union_r.
+      rewrite <- subst_BoundVar_f_eq_subdomain.
+      eapply f_eq_subdomain_extend_not_In_S_l.
+      intros H. eapply Hd. constructor. rewrite FromList_cons.
+      now left. eassumption.
+      eapply IHl. eapply Disjoint_Included_l; [| eassumption ].
+      rewrite FromList_cons. now apply Included_Union_r.
+  Qed.
+
+  Lemma exp_closure_conv_Closure_conv_sound :
+    (forall e Scope Funs Γ FVs FVmap S
+       (* The invariant the relates [FVmap] and [Scope], [Funs], [FV] *)
+       (Minv : FVmap_inv FVmap Scope Funs FVs)
+       (* [FVmap] contains all the free variables *)
+       (Hbin1 : binding_in_map (occurs_free e) FVmap)
+       (* [FVmap] does not contain the variables in [S] or [Γ] *)
+       (Hbin2 : binding_not_in_map (Union _ S (Singleton _ Γ)) FVmap)
+       (* [S] is disjoint with the free and bound variables of [e] and [Γ] *)
+       (HD1 : Disjoint _ S (Union _ (image (subst FVmap) (Setminus _ Funs Scope))
+                                  (Union _ (bound_var e)
+                                         (Union _ (occurs_free e) (Singleton _ Γ)))))
+       (* The current environment argument is fresh *)
+       (HD2 : ~ In _ (Union _ (bound_var e) (occurs_free e)) Γ),
+       {{ fun s => True }}
+         exp_closure_conv utag env_tag tag_bij unknown_type e FVmap Γ
+       {{ fun s ef s' =>
+            fresh S (fst s) ->
+            exists C, is_exp_ctx (snd ef) C /\
+                 Closure_conversion Scope Funs (subst FVmap) Γ FVs e (fst ef) C /\
+                 fresh S (fst s')
+       }}) /\
+    (forall B FVmap Funs FVs S
+       (Minv : FVmap_inv FVmap (Empty_set _) Funs FVs)
+       (Hbin1 : binding_in_map (Union _ (occurs_free_fundefs B) (name_in_fundefs B)) FVmap)
+       (Hbin2 : binding_not_in_map S FVmap)
+       (HD1 : Disjoint _ S (Union _ (image (subst FVmap) Funs)
+                                  (Union _ (bound_var_fundefs B) (occurs_free_fundefs B))))
+       (Hinc : Included _ (name_in_fundefs B) Funs),
+       {{ fun s => True }}
+         fundefs_closure_conv utag env_tag tag_bij unknown_type B FVmap
+       {{ fun s B' s' =>
+            fresh S (fst s) ->       
+            Closure_conversion_fundefs Funs (subst FVmap) FVs B B' /\
+            fresh S (fst s')
+       }}).
+  Proof.
+    eapply exp_def_mutual_ind; intros.
+    - eapply pre_post_mp_r. eapply bind_triple.
+      + eapply get_vars_project_vars_sound; [ | eassumption ].
+        intros x Hx. eapply Hbin1. eauto.
+      + intros [xs f] s. eapply pre_eq_state.
+        intros [x'' d''] [C [S' [Hf [Hproj Hctx]]]].
+        eapply pre_post_mp_l.
+        eapply bind_triple.
+        eapply H with (Scope := Union var (Singleton var v) Scope)
+                      (S := S')
+                      (FVmap := Maps.PTree.set v (BoundVar t) FVmap).
+        * eapply FVmap_inv_set_bound. eassumption. 
+        * eapply binding_in_map_antimon; [| eapply binding_in_map_set; eassumption ].
+          now eapply occurs_free_Econstr_Included.
+        * eapply binding_not_in_map_antimon. 
+          apply Included_Union_compat. eapply project_vars_free_set_Included; now eauto. 
+          now apply Included_refl.
+          eapply binding_not_in_map_set_not_In_S. eassumption.
+          intros Hc; inv Hc. now eapply HD1; eauto. inv H0; eapply HD2; eauto.
+        * eapply Disjoint_Included_l. eapply project_vars_free_set_Included; now eauto.
+          eapply Disjoint_Included_r; [| eassumption ].
+          apply Included_Union_compat.
+          rewrite <- subst_BoundVar_f_eq.
+          rewrite Union_sym, <- Setminus_Union. now eapply image_Setminus_extend.
+          rewrite !Union_assoc.
+          apply Included_Union_compat; [| now apply Included_refl ].
+          now apply bound_var_occurs_free_Econstr_Included.
+        * intros Hc. inv Hc; eapply HD2; eauto.
+          rewrite bound_var_Econstr, occurs_free_Econstr. 
+          destruct (Coqlib.peq Γ v); subst. now eauto.
+          right. right. constructor; eauto. intros Hc; inv Hc. congruence.
+        * intros e' s'. eapply return_triple. intros s'' Hf' Hcc. subst.
+          edestruct (Hf' Hf) as [C' [Hctx' [Hcc Hf'']]]; eauto.
+          do 2 eexists. eapply Hctx. split.
+          simpl. rewrite Hctx'. econstructor. eapply Disjoint_free_set in Minv.  
+          eapply Disjoint_sym. eapply Disjoint_Union; eapply Disjoint_sym.
+          eapply Disjoint_Included_r; [| eassumption ]. now apply Included_Union_l.
+          eapply Disjoint_sym. eapply Disjoint_Union; eapply Disjoint_sym.
+          eapply Disjoint_Included_r; [| now apply HD1 ]. now apply Included_Union_l.
+          eapply Disjoint_sym. eapply Disjoint_Union; eapply Disjoint_sym.
+          eapply Disjoint_Included_r; [| eassumption ]. apply Included_Union_mon_r.
+          now apply Included_Union_r.
+          eapply Disjoint_Included_r; [| now apply HD1 ]. do 3 apply Included_Union_mon_r.
+          now apply Included_refl.
+          eapply binding_not_in_map_antimon; [| eassumption ]. now apply Included_Union_l.
+          eassumption.
+          eapply Closure_conversion_f_eq_subdomain. eassumption.
+          rewrite <- subst_BoundVar_f_eq. apply f_eq_subdomain_extend_not_In_S_l.
+          intros Hc. inv Hc. now eauto. reflexivity.
+          eapply fresh_monotonic. now eapply project_vars_free_set_Included; eauto.
+          eassumption.
+    - eapply pre_post_mp_r. eapply bind_triple with (post' := fun _ l i => l = [] /\ fresh S (fst i)).
+      + eapply return_triple; eauto. 
+      + intros pats' s2.
+        eapply bind_triple.
+        * eapply frame_rule. eapply get_var_project_var_sound; eauto.
+          intros x Hx. eapply Hbin1. rewrite occurs_free_Ecase_nil. eassumption.
+        * intros [[x tau] f] s. eapply return_triple.
+          intros s' [Heq [C [S' [Hf [Hproj Hctx]]]]]. rewrite Heq.
+          eexists. split; eauto. split. econstructor; [| eassumption |].
+          eapply Disjoint_free_set in Minv.
+          eapply Disjoint_sym. eapply Disjoint_Union; eapply Disjoint_sym.
+          eapply Disjoint_Included_r; [| eassumption ]. now apply Included_Union_l.
+          eapply Disjoint_sym. eapply Disjoint_Union; eapply Disjoint_sym.
+          eapply Disjoint_Included_r; [| now apply HD1 ]. now apply Included_Union_l.
+          eapply Disjoint_sym. eapply Disjoint_Union; eapply Disjoint_sym.
+          eapply Disjoint_Included_r; [| eassumption ]. apply Included_Union_mon_r.
+          now apply Included_Union_r.
+          eapply Disjoint_Included_r; [| now apply HD1 ]. do 3 apply Included_Union_mon_r.
+          now apply Included_refl.
+          eapply binding_not_in_map_antimon; [| eassumption ]. now apply Included_Union_l.
+          now constructor.
+          eapply fresh_monotonic. now eapply project_var_free_set_Included; eauto.
+          eassumption.
+    - unfold exp_closure_conv. setoid_rewrite assoc.
+      eapply bind_triple.
+      + eapply H; [ eassumption | | eassumption | | ].
+        * eapply binding_in_map_antimon; [| eassumption ].
+          eapply occurs_free_Ecase_Included. now constructor.
+        * eapply Disjoint_Included_r; [| eassumption ].
+          apply Included_Union_compat. now apply Included_refl.
+          rewrite !Union_assoc. apply Included_Union_compat; [| now apply Included_refl ].
+          eapply bound_var_occurs_free_Ecase_Included. now constructor. 
+        * intros Hc. apply HD2.
+          rewrite bound_var_Ecase_cons, occurs_free_Ecase_cons.
+          inv Hc; eauto.
+      + intros [e' f'] s'. simpl. setoid_rewrite assoc. simpl.
+        setoid_rewrite st_eq_Ecase. 
+        eapply pre_post_mp_l. eapply bind_triple. 
+        eapply H0 with (FVmap := FVmap) (Γ := Γ);
+          [ eassumption | | eassumption | | ].
+        * eapply binding_in_map_antimon; [| eassumption ].
+          rewrite occurs_free_Ecase_cons. apply Included_Union_mon_r.
+          now apply Included_Union_r.
+        * eapply Disjoint_Included_r; [| eassumption ].
+          apply Included_Union_compat. now apply Included_refl.
+          rewrite !Union_assoc. apply Included_Union_compat; [| now apply Included_refl ].
+          eapply bound_var_occurs_free_Ecase_cons_Included.
+        * intros Hc. apply HD2.
+          rewrite bound_var_Ecase_cons, occurs_free_Ecase_cons.
+          inv Hc; eauto.
+        * intros [e'' f s''].   
+          edestruct e''; eapply return_triple; intros s''' Hcc1 Hcc2 Hf;
+          edestruct (Hcc2 Hf) as [C2 [Hctx2 [Hcc2'  Hf2]]];
+          edestruct (Hcc1 Hf2) as [C1 [Hctx1 [Hcc1' Hf1]]]; inv Hcc1'.
+          eexists. repeat split.
+          eassumption.
+          simpl. econstructor; [ eassumption | eassumption | now constructor; eauto ].
+          eassumption.
+    - eapply pre_post_mp_r. eapply bind_triple.
+      + eapply get_var_project_var_sound; [ | eassumption ].
+        intros x Hx. inv Hx. eapply Hbin1. eauto.
+      + intros [[x tau] f] s. eapply pre_eq_state.
+        intros [x'' d''] [C [S' [Hf [Hproj Hctx]]]].
+        eapply pre_post_mp_l.
+        eapply bind_triple.
+        eapply H with (Scope := Union var (Singleton var v) Scope)
+                      (S := S')
+                      (FVmap := Maps.PTree.set v (BoundVar t) FVmap).
+        * eapply FVmap_inv_set_bound. eassumption. 
+        * eapply binding_in_map_antimon; [| eapply binding_in_map_set; eassumption ].
+          now eapply occurs_free_Eproj_Included.
+        * eapply binding_not_in_map_antimon.
+          apply Included_Union_compat. now eapply project_var_free_set_Included; eauto.
+          now apply Included_refl.
+          eapply binding_not_in_map_set_not_In_S. eassumption.
+          intros Hc; inv Hc. now eapply HD1; eauto. inv H0; eapply HD2; eauto.
+        * eapply Disjoint_Included_l. eapply project_var_free_set_Included; now eauto.
+          eapply Disjoint_Included_r; [| eassumption ].
+          apply Included_Union_compat.
+          rewrite <- subst_BoundVar_f_eq.
+          rewrite Union_sym, <- Setminus_Union. now eapply image_Setminus_extend.
+          rewrite !Union_assoc.
+          apply Included_Union_compat; [| now apply Included_refl ].
+          now apply bound_var_occurs_free_Eproj_Included.
+        * intros Hc. inv Hc; eapply HD2; eauto.
+          rewrite bound_var_Eproj, occurs_free_Eproj. 
+          destruct (Coqlib.peq Γ v); subst. now eauto.
+          right. right. constructor; eauto. intros Hc; inv Hc. congruence.
+        * intros e' s'. eapply return_triple. intros s'' Hf' Hcc. subst.
+          edestruct (Hf' Hf) as [C' [Hctx' [Hcc Hf'']]]; eauto.
+          do 2 eexists. eapply Hctx. split.
+          simpl. rewrite Hctx'. econstructor. eapply Disjoint_free_set in Minv.  
+          eapply Disjoint_sym. eapply Disjoint_Union; eapply Disjoint_sym.
+          eapply Disjoint_Included_r; [| eassumption ]. now apply Included_Union_l.
+          eapply Disjoint_sym. eapply Disjoint_Union; eapply Disjoint_sym.
+          eapply Disjoint_Included_r; [| now apply HD1 ]. now apply Included_Union_l.
+          eapply Disjoint_sym. eapply Disjoint_Union; eapply Disjoint_sym.
+          eapply Disjoint_Included_r; [| eassumption ]. apply Included_Union_mon_r.
+          now apply Included_Union_r.
+          eapply Disjoint_Included_r; [| now apply HD1 ]. do 3 apply Included_Union_mon_r.
+          now apply Included_refl.
+          eapply binding_not_in_map_antimon; [| eassumption ]. now apply Included_Union_l.
+          eassumption.
+          eapply Closure_conversion_f_eq_subdomain. eassumption.
+          rewrite <- subst_BoundVar_f_eq. apply f_eq_subdomain_extend_not_In_S_l.
+          intros Hc. inv Hc. now eauto. reflexivity.
+          eapply fresh_monotonic. now eapply project_var_free_set_Included; eauto.
+          eassumption.
+    - eapply pre_post_mp_r. eapply bind_triple; [ now eapply get_name_fresh |].
+      intros Γ' s1. eapply pre_uncurry_l. intros Hf1.
+      eapply bind_triple.
+      + eapply make_env_spec. eapply binding_in_map_antimon; [| eassumption ].
+        * intros x Hfv. eapply occurs_free_Efun. left.
+          eapply fundefs_fv_correct. eassumption. 
+        * eapply binding_not_in_map_antimon; [| eassumption ].
+          eapply Included_Union_compat. now apply Subset_Setminus.
+          now apply Included_refl.
+        * eassumption.
+      + intros [[tau FVmap'] f] _. eapply pre_existential; intros C1.
+        eapply pre_existential; intros S2. eapply pre_existential; intros FVs'.
+        eapply pre_existential; intros tau'. eapply pre_existential; intros t.
+        eapply pre_uncurry_r. intros [Hproj [Hctx1 [Hb1 [Hb1' Minv1]]]].
+        eapply bind_triple; [ eapply make_full_closure_spec; eassumption |].
+        intros [[FVmap_n FVmap_o] f'] s2. eapply pre_existential; intros C2.
+        eapply pre_existential; intros S3. eapply pre_uncurry_r.
+        intros [Hmc [Hctx2 [Hfeq [Hb2 [Hb2' [Hb3 [Hb3' [Minv_n Minv_o]]]]]]]].
+        eapply pre_post_mp_l. eapply bind_triple.
+        * eapply H0 with (S := S3) ; [ eassumption | | | | ].
+          eapply binding_in_map_antimon; [| eassumption ].
+          now apply occurs_free_Efun_Included.
+          eapply binding_not_in_map_antimon; [| eassumption ].
+          rewrite <- Included_Setminus_Disjoint.
+          eapply Included_Union_compat.
+          eapply Included_trans. eapply Included_trans. now eapply make_closures_free_set_Included; eauto.
+          now eapply project_vars_free_set_Included; eauto. now apply Subset_Setminus.
+          now apply Included_refl.
+          eapply Disjoint_Union.
+          eapply Disjoint_Included_r; [| eassumption ].
+          apply Included_Union_mon_r. apply Included_Union_mon_l.
+          rewrite bound_var_Efun. apply Included_Union_mon_l. now apply name_in_fundefs_bound_var_fundefs.
+          apply Disjoint_sym. eapply Disjoint_Singleton. intros Hc. eapply HD2.
+          left. rewrite bound_var_Efun. left. now apply name_in_fundefs_bound_var_fundefs.
+          eapply Disjoint_Included_r; [| eapply Disjoint_Included_l; [| eassumption ] ].
+          eapply Included_Union_compat. rewrite Union_sym. rewrite <- image_f_eq_subdomain. 
+          apply image_monotonic. apply Included_Setminus_compat. now apply Included_refl.
+          now apply Included_Union_l. eassumption. 
+          rewrite !Union_assoc. eapply Included_Union_compat.
+          now apply bound_var_occurs_free_Efun_Included. now apply Included_refl.
+          eapply Included_trans. eapply Included_trans. now eapply make_closures_free_set_Included; eauto.
+          now eapply project_vars_free_set_Included; eauto. now apply Subset_Setminus.
+          intros H'. eapply HD2. now eapply bound_var_occurs_free_Efun_Included.
+        * intros [e' f''] s3. eapply pre_post_mp_l.
+          eapply bind_triple.
+          eapply H. eassumption. eapply binding_in_map_antimon; [| eassumption ].
+          apply Included_Union_compat. rewrite fundefs_fv_correct.
+          now apply Included_refl. now apply Included_refl.          
+          eapply binding_not_in_map_antimon with (S' := S3); [| eassumption ].
+          eapply Included_trans. eapply Included_trans. eapply Included_trans.
+          now eapply make_closures_free_set_Included; eauto.
+          now eapply project_vars_free_set_Included; eauto.          
+          now apply Subset_Setminus.
+          intros x H'. constructor. intros Hc.
+          eapply HD1. constructor. now eauto. do 2 right. left. rewrite occurs_free_Efun.
+          left. eapply fundefs_fv_correct. eassumption. intros Hc. eapply HD1. constructor. now eauto.
+          right. left. rewrite bound_var_Efun. left. now apply name_in_fundefs_bound_var_fundefs.
+          eapply Disjoint_sym. eapply Disjoint_Union.
+          eapply make_closures_image_Disjoint. eassumption.  
+          apply Disjoint_sym.
+          eapply Disjoint_Included_l. now eapply make_closures_free_set_Included; eauto.
+          eapply Disjoint_Included_l. now eapply project_vars_free_set_Included; eauto.
+          eapply Disjoint_Included_l. now eapply Subset_Setminus.
+          eapply Disjoint_Included_r; [| eassumption ].
+          apply Included_Union_mon_r. rewrite Union_assoc.
+          apply Included_Union_mon_l. now apply bound_var_occurs_free_fundefs_Efun_Included.
+          now apply Included_refl.
+          intros B s4. apply return_triple. intros s5 H1 H2 H3.
+          edestruct (H2 H3) as [C'' [Hctx'' [Hcc'' Hf'']]]; eauto.
+          edestruct (H1 Hf'') as [Hcc' Hf']; eauto.
+          eexists.  split. eassumption. 
+          split. simpl. rewrite Hctx'', Hctx2.
+          assert (HD3 :
+                    Disjoint M.elt S
+                             (Union var (bound_var_fundefs f2)
+                                    (Union var Scope
+                                           (Union var (image (subst FVmap) (Setminus var Funs Scope))
+                                                  (Union var (FromList FVs) (Singleton var Γ)))))).
+          { eapply Disjoint_free_set in Minv.  
+            eapply Disjoint_sym. eapply Disjoint_Union; eapply Disjoint_sym.
+            eapply Disjoint_Included_r; [| now eapply HD1 ]. 
+            apply Included_Union_mon_r. apply Included_Union_mon_l.
+            rewrite bound_var_Efun. now apply Included_Union_l.
+            eapply Disjoint_sym. eapply Disjoint_Union; eapply Disjoint_sym.
+            eapply Disjoint_Included_r; [| eassumption ]. now apply Included_Union_l.
+            eapply Disjoint_sym. eapply Disjoint_Union; eapply Disjoint_sym.
+            eapply Disjoint_Included_r; [| now apply HD1 ]. now apply Included_Union_l.
+            eapply Disjoint_sym. eapply Disjoint_Union; eapply Disjoint_sym.
+            eapply Disjoint_Included_r; [|  eassumption ]. apply Included_Union_mon_r.
+            now apply Included_Union_r.
+            eapply Disjoint_Included_r; [| now apply HD1 ]. do 3 apply Included_Union_mon_r.
+            now apply Included_refl.
+            eapply binding_not_in_map_antimon; [| eassumption ]. now apply Included_Union_l. }
+          econstructor; [ | | eassumption | | eassumption | | eassumption | eassumption |  ].
+          now eapply fundefs_fv_correct.
+          eapply Disjoint_Included_l. now apply Subset_Setminus. 
+          eapply Disjoint_Included_r; [| eassumption ].
+          now apply Included_Union_r.
+          eapply Disjoint_Included_l with (s8 := S).
+          intros x Hin. eapply Hin. zify. omega. eapply Disjoint_Included_r; [| eassumption ]. 
+          eapply Included_Union_compat. now apply name_in_fundefs_bound_var_fundefs.
+          now apply Included_refl.
+          rewrite Union_assoc, (Union_sym _ (Singleton var Γ')), <- Union_assoc.
+          eapply Disjoint_sym. eapply Disjoint_Union; eapply Disjoint_sym.
+          eapply Disjoint_Included_l.
+          eapply project_vars_free_set_Included; eassumption.
+          eapply Disjoint_Setminus. now apply Included_refl.
+          eapply Disjoint_Included_l.
+          eapply Included_trans. eapply project_vars_free_set_Included; eassumption.
+          now apply Subset_Setminus. eassumption.
+          eapply Closure_conversion_f_eq_subdomain. eassumption.
+          rewrite Union_sym. symmetry. eassumption.
+          eapply fresh_monotonic; [ | eassumption ].
+          eapply Included_trans. eapply Included_trans.
+          now eapply make_closures_free_set_Included; eauto.
+          now eapply project_vars_free_set_Included; eauto. now apply Subset_Setminus.
+    - eapply pre_post_mp_r. eapply bind_triple.
+      + eapply get_var_project_var_sound; [  | eassumption ].
+        eapply binding_in_map_antimon; [| eassumption ].
+        rewrite occurs_free_Eapp. apply Included_Union_mon_r.
+        now apply Included_refl.
+      + intros [[x tau] f] s1. eapply pre_existential. intros C1.
+        eapply pre_existential. intros S'.
+        eapply pre_uncurry_r. intros [Hvar Hctx1].
+        eapply bind_triple.
+        * eapply get_vars_project_vars_sound; [ | eassumption ].
+          eapply binding_in_map_antimon; [| eassumption ].
+          rewrite occurs_free_Eapp. apply Included_Union_mon_l.
+          now apply Included_refl.
+        * intros [xs f'] s2. eapply pre_existential. intros C2.
+          eapply pre_existential. intros S''.
+          eapply pre_uncurry_r. intros [Hvars  Hctx2]. eapply bind_triple.
+          eapply get_name_fresh.
+          intros x' i. eapply pre_uncurry_l. intros Hf1.
+          eapply bind_triple.
+          now eapply get_name_fresh. 
+          intros x'' s3. eapply pre_uncurry_l. intros Hf2. 
+          eapply bind_triple. eapply get_typeinfo_preserves_prop.
+          intros tinf s4. eapply return_triple.
+          intros s5 Hf5. simpl. exists (comp_ctx_f C1 C2).
+          split. intros e. rewrite <- app_ctx_f_fuse. congruence.
+          split; eauto.
+          econstructor;
+            [ | econstructor; eassumption | eapply Hf1; now apply Pos.le_refl
+              | eapply Hf2; now apply Pos.le_refl
+              | intros Hc; subst x';  eapply Hf2;
+                [ now apply Pos.le_refl | now eauto ]].
+          eapply Disjoint_free_set in Minv.
+          eapply Disjoint_sym. eapply Disjoint_Union; eapply Disjoint_sym.
+          eapply Disjoint_Included_r; [| eassumption ]. now apply Included_Union_l.
+          eapply Disjoint_sym. eapply Disjoint_Union; eapply Disjoint_sym.
+          eapply Disjoint_Included_r; [| now apply HD1 ]. now apply Included_Union_l.
+          eapply Disjoint_sym. eapply Disjoint_Union; eapply Disjoint_sym.
+          eapply Disjoint_Included_r; [| eassumption ]. apply Included_Union_mon_r.
+          now apply Included_Union_r.
+          eapply Disjoint_Included_r; [| now apply HD1 ]. do 3 apply Included_Union_mon_r.
+          now apply Included_refl.
+          eapply binding_not_in_map_antimon; [| eassumption ]. now apply Included_Union_l.
+          eapply fresh_monotonic; [| eassumption ].
+          do 2 (eapply Included_trans; [ now apply Subset_Setminus |]).
+          eapply Included_trans. now eapply project_vars_free_set_Included; eauto.
+          eapply Included_trans. now eapply project_var_free_set_Included; eauto.
+          now apply Included_refl.
+    - eapply pre_post_mp_r. eapply bind_triple.
+      + eapply get_vars_project_vars_sound; [ | eassumption ].
+        intros x Hx. eapply Hbin1. eauto.
+      + intros [xs f] s. eapply pre_eq_state.
+        intros [x'' d''] [C [S' [Hf [Hproj Hctx]]]].
+        eapply pre_post_mp_l.
+        eapply bind_triple.
+        eapply H with (Scope := Union var (Singleton var v) Scope)
+                      (S := S')
+                      (FVmap := Maps.PTree.set v (BoundVar t) FVmap).
+        * eapply FVmap_inv_set_bound. eassumption. 
+        * eapply binding_in_map_antimon; [| eapply binding_in_map_set; eassumption ].
+          now eapply occurs_free_Eprim_Included.
+        * eapply binding_not_in_map_antimon. 
+          apply Included_Union_compat. eapply project_vars_free_set_Included; now eauto. 
+          now apply Included_refl.
+          eapply binding_not_in_map_set_not_In_S. eassumption.
+          intros Hc; inv Hc. now eapply HD1; eauto. inv H0; eapply HD2; eauto.
+        * eapply Disjoint_Included_l. eapply project_vars_free_set_Included; now eauto.
+          eapply Disjoint_Included_r; [| eassumption ].
+          apply Included_Union_compat.
+          rewrite <- subst_BoundVar_f_eq.
+          rewrite Union_sym, <- Setminus_Union. now eapply image_Setminus_extend.
+          rewrite !Union_assoc.
+          apply Included_Union_compat; [| now apply Included_refl ].
+          now apply bound_var_occurs_free_Eprim_Included.
+        * intros Hc. inv Hc; eapply HD2; eauto.
+          rewrite bound_var_Eprim, occurs_free_Eprim. 
+          destruct (Coqlib.peq Γ v); subst. now eauto.
+          right. right. constructor; eauto. intros Hc; inv Hc. congruence.
+        * intros e' s'. eapply return_triple. intros s'' Hf' Hcc. subst.
+          edestruct (Hf' Hf) as [C' [Hctx' [Hcc Hf'']]]; eauto.
+          do 2 eexists. eapply Hctx. split.
+          simpl. rewrite Hctx'. econstructor. eapply Disjoint_free_set in Minv.  
+          eapply Disjoint_sym. eapply Disjoint_Union; eapply Disjoint_sym.
+          eapply Disjoint_Included_r; [| eassumption ]. now apply Included_Union_l.
+          eapply Disjoint_sym. eapply Disjoint_Union; eapply Disjoint_sym.
+          eapply Disjoint_Included_r; [| now apply HD1 ]. now apply Included_Union_l.
+          eapply Disjoint_sym. eapply Disjoint_Union; eapply Disjoint_sym.
+          eapply Disjoint_Included_r; [| eassumption ]. apply Included_Union_mon_r.
+          now apply Included_Union_r.
+          eapply Disjoint_Included_r; [| now apply HD1 ]. do 3 apply Included_Union_mon_r.
+          now apply Included_refl.
+          eapply binding_not_in_map_antimon; [| eassumption ]. now apply Included_Union_l.
+          eassumption.
+          eapply Closure_conversion_f_eq_subdomain. eassumption.
+          rewrite <- subst_BoundVar_f_eq. apply f_eq_subdomain_extend_not_In_S_l.
+          intros Hc. inv Hc. now eauto. reflexivity.
+          eapply fresh_monotonic. now eapply project_vars_free_set_Included; eauto.
+          eassumption.
+    - assert (Hincl : Included var (Union var (bound_var e) (occurs_free e))
+                               (Union var (bound_var_fundefs (Fcons v t l e f5))
+                                      (occurs_free_fundefs (Fcons v t l e f5)))).
+      { rewrite bound_var_fundefs_Fcons.
+        rewrite !Union_assoc,
+        Union_sym with (s2 := FromList l), Union_sym with (s2 := bound_var e), <- !Union_assoc.
+        apply Included_Union_compat. now apply Included_refl.
+        eapply Included_trans. eapply occurs_free_in_fun with (B := Fcons v t l e f5).
+        econstructor. now eauto. apply Included_Union_compat. now apply Included_refl. 
+        simpl. rewrite <- Union_assoc. apply Included_Union_compat. now apply Included_refl. 
+        apply Included_Union_compat; [| now apply Included_refl ].
+        now eapply name_in_fundefs_bound_var_fundefs. }
+      eapply pre_post_mp_r. eapply bind_triple.
+      now apply get_typeinfo_preserves_prop.
+      intros tau s1. eapply bind_triple. now apply get_name_fresh.
+      intros x s2. apply pre_uncurry_l. intros Hf1. 
+      eapply pre_post_mp_l. eapply bind_triple.
+      eapply H with (Scope := FromList l) (Funs := Funs) (FVs := FVs) (S := Setminus _ S (Singleton _ x)).
+      + rewrite <- Union_Empty_set_r with (s := FromList l). eapply FVmapInv_add_params.
+        eassumption.
+      + eapply binding_in_map_antimon; [| eapply binding_in_map_add_params; eassumption ].
+        rewrite Union_sym. rewrite Union_sym with (s3 := occurs_free_fundefs _ ).
+        eapply occurs_free_in_fun. constructor. eauto.
+      + intros x'. rewrite <- (@Union_Setminus _ _ _ _), Union_Included_Same_set. 
+        eapply binding_not_in_map_add_params. eassumption.
+        constructor. intros y Hc. inv Hc. eapply HD1. constructor; eauto. now right; eauto.
+        intros x'' Hc; inv Hc. eapply Hf1. zify; omega.
+      + rewrite !Union_assoc. apply Disjoint_sym. apply Disjoint_Union; apply Disjoint_sym.
+        eapply Disjoint_Included_l. now apply Subset_Setminus.
+        eapply Disjoint_Included_r; [| eassumption ]. rewrite <- !Union_assoc.
+        apply Included_Union_compat. rewrite image_f_eq_subdomain.
+        apply image_monotonic. now apply Subset_Setminus.
+        apply subst_add_params_f_eq_subdomain. eapply Disjoint_sym. eapply Disjoint_Setminus.
+        now apply Included_refl. eassumption.
+        now eapply Disjoint_Setminus.
+      + intros Hc. eapply HD1. inv Hc.
+        constructor; [ | now eauto ]; eapply Hf1; zify; omega.
+        constructor. eapply Hf1; zify; omega. right.
+        eapply occurs_free_in_fun with (B := Fcons v t l e f5) in H1; [| econstructor; now eauto ].
+        inv H1; eauto. inv H2; eauto. left. now eapply name_in_fundefs_bound_var_fundefs. 
+      + intros [e' f] s3. eapply pre_post_mp_l. eapply bind_triple.
+        eapply H0 with (S := Setminus _ S (Singleton _ x)); [ eassumption | | | | ].
+        * eapply binding_in_map_antimon; [| eassumption ].
+          simpl. rewrite Union_assoc. apply Included_Union_compat.
+          now apply occurs_free_fundefs_Fcons_Included. now apply Included_refl.
+        * eapply binding_not_in_map_antimon. now apply Subset_Setminus.
+          eassumption.
+        * eapply Disjoint_Included_l. now apply Subset_Setminus.
+          eapply Disjoint_Included_r; [| eassumption ].
+          apply Included_Union_compat. now apply Included_refl.
+          rewrite bound_var_fundefs_Fcons. rewrite Union_sym with (s4 := Singleton var v).
+          do 2 rewrite <- Union_assoc. rewrite Union_sym with (s4 := Singleton var v).
+          apply Included_Union_mon_r. (* TODO lemma *)
+          apply Included_Union_compat. now apply Included_Union_r.
+          now apply occurs_free_fundefs_Fcons_Included.
+        * eapply Included_trans; [| eassumption ]. now apply Included_Union_r.
+        * intros B' s5.
+          assert (Ha: exists v' tau1 tau2, Maps.PTree.get v FVmap = Some (MRFun v' tau1 tau2)).
+          { destruct Minv as [_ [HM _]]. eapply HM. rewrite Setminus_Empty_set_Same_set.
+            eapply Hinc. left; eauto. }
+          destruct Ha as [v' [tau1 [tau2 Ha']]]. rewrite Ha'.
+          eapply return_triple. intros s6 Hcc1 Hcc2 Hf. 
+          edestruct (Hcc2 Hf) as [C1 [Hctx1 [Hcc1' Hf1']]].
+          destruct (Hcc1 Hf1') as [Hcc2' Hf2'].
+          split; [| eapply fresh_monotonic; [ now apply Subset_Setminus | eassumption ]].
+          simpl. rewrite Hctx1.
+          replace v' with ((subst FVmap) v) by (unfold subst; rewrite Ha'; reflexivity).
+          econstructor; [| eassumption | eassumption |].
+          eapply (Disjoint_Included_l _ _ S). intros x' Hx'. eapply Hx'. zify; omega.
+          eapply Disjoint_Included_r; [| eassumption ].
+          apply Included_Union_compat. now apply Included_refl.
+          apply Included_Union_mon_l. rewrite bound_var_fundefs_Fcons.
+          apply Included_Union_mon_r. apply Included_Union_compat. now apply Included_refl.
+          now apply Included_Union_l.
+          eapply Closure_conversion_f_eq_subdomain. eassumption.
+          eapply subst_add_params_f_eq_subdomain.
+          eapply Disjoint_sym. eapply Disjoint_Setminus. now apply Included_refl.
+    - eapply return_triple. intros Hc _ Hf.
+      split; [| eassumption ]. constructor.
+  Qed.
+
+End CC_correct.
